improve consistency between c word and set game

Contrasim_Word_Game.thy
@@ -1,67 +1,67 @@
-section \<open>The Basic Contrasimulation Preorder Game\<close>
+section \<open>The Contrasimulation Preorder Word Game\<close>
 
-theory Basic_Contrasim_Game
+theory Contrasim_Word_Game
 imports
   Simple_Game
   Contrasimulation
 begin
 
-datatype ('s, 'a) c_basic_game_node =
+datatype ('s, 'a) c_word_game_node =
   AttackerNode 's 's |
   DefenderNode "'a list" 's 's
 
-fun (in lts_tau) c_game_moves ::
-  \<open>('s, 'a) c_basic_game_node \<Rightarrow> ('s, 'a) c_basic_game_node \<Rightarrow> bool\<close> where
+fun (in lts_tau) c_word_game_moves ::
+  \<open>('s, 'a) c_word_game_node \<Rightarrow> ('s, 'a) c_word_game_node \<Rightarrow> bool\<close> where
                              
   simulation_challenge:
-   \<open>c_game_moves (AttackerNode p q) (DefenderNode A p1 q0) =
+   \<open>c_word_game_moves (AttackerNode p q) (DefenderNode A p1 q0) =
      (p \<Rightarrow>$A p1 \<and> q = q0 \<and> (\<forall>a\<in>set A. a \<noteq> \<tau>))\<close> |     
 
   simulation_answer:                        
-    \<open>c_game_moves (DefenderNode A p1 q0) (AttackerNode q1 p10) =
+    \<open>c_word_game_moves (DefenderNode A p1 q0) (AttackerNode q1 p10) =
       (q0 \<Rightarrow>$A q1 \<and> p1 = p10)\<close> |                                             
                                              
-  c_game_moves_no_step:               
-    \<open>c_game_moves _ _ = False\<close>
+  c_word_game_moves_no_step:               
+    \<open>c_word_game_moves _ _ = False\<close>
 
-fun c_game_defender_node :: \<open>('s, 'a) c_basic_game_node \<Rightarrow> bool\<close> where
-  \<open>c_game_defender_node (AttackerNode _ _) = False\<close> |
-  \<open>c_game_defender_node (DefenderNode _ _ _) = True\<close>
+fun c_word_game_defender_node :: \<open>('s, 'a) c_word_game_node \<Rightarrow> bool\<close> where
+  \<open>c_word_game_defender_node (AttackerNode _ _) = False\<close> |
+  \<open>c_word_game_defender_node (DefenderNode _ _ _) = True\<close>
 
 
-subsection \<open>Contrasimulation Implies Winning Strategy (Completeness)\<close>
+subsection \<open>Contrasimulation Implies Winning Strategy in Word Game (Completeness)\<close>
 
-locale c_basic_game =
+locale c_word_game =
   lts_tau trans \<tau> +
-  simple_game c_game_moves c_game_defender_node
+  simple_game c_word_game_moves c_word_game_defender_node
 for
   trans :: \<open>'s \<Rightarrow> 'a \<Rightarrow> 's \<Rightarrow> bool\<close> and
   \<tau> :: \<open>'a\<close> and 
-  initial :: \<open>('s, 'a) c_basic_game_node\<close> 
+  initial :: \<open>('s, 'a) c_word_game_node\<close> 
 begin
 
-fun strategy_from_contrasim:: \<open>('s \<Rightarrow> 's \<Rightarrow> bool) \<Rightarrow> ('s, 'a) c_basic_game_node strategy\<close> where
+fun strategy_from_contrasim:: \<open>('s \<Rightarrow> 's \<Rightarrow> bool) \<Rightarrow> ('s, 'a) c_word_game_node strategy\<close> where
   \<open>strategy_from_contrasim R ((DefenderNode A p1 q0)#play) =
     (AttackerNode (SOME q1 . R q1 p1 \<and> q0 \<Rightarrow>$A q1) p1)\<close> |
   \<open>strategy_from_contrasim _ _ = undefined\<close>
 
-lemma bcg_atknodes_precede_defnodes_in_plays: 
+lemma cwg_atknodes_precede_defnodes_in_plays: 
   assumes 
-    \<open>c_game_defender_node n0\<close>
+    \<open>c_word_game_defender_node n0\<close>
     \<open>n0 = DefenderNode A p' q\<close>
     \<open>(n0#play) \<in> plays initial\<close>
     \<open>initial = AttackerNode p0 q0\<close>
-  shows \<open>\<exists>p. (hd play) = AttackerNode p q \<and> c_game_moves (hd play) n0\<close>
+  shows \<open>\<exists>p. (hd play) = AttackerNode p q \<and> c_word_game_moves (hd play) n0\<close>
 proof -
   have \<open>n0 \<noteq> initial\<close> using assms (2, 4) by auto
-  hence mov: \<open>c_game_moves (hd play) n0\<close> using assms(3)
+  hence mov: \<open>c_word_game_moves (hd play) n0\<close> using assms(3)
     by (metis list.inject list.sel(1) plays.cases)     
   hence \<open>\<exists>p. (hd play) = AttackerNode p q\<close> using assms(1 - 3)
-    by (metis c_basic_game_node.inject(2) c_game_defender_node.simps(1) c_game_moves.elims(2))
+    by (metis c_word_game_node.inject(2) c_word_game_defender_node.simps(1) c_word_game_moves.elims(2))
   thus ?thesis using mov by auto
 qed
 
-lemma bcg_second_play_elem_in_play_set : 
+lemma cwg_second_play_elem_in_play_set : 
   assumes 
     \<open>(n0#play) \<in> plays initial\<close>
     \<open>initial = AttackerNode p0 q0\<close>
@@ -78,7 +78,7 @@ proof -
   with x_in_set show \<open>hd play \<in> set (n0 # play)\<close> by auto
 qed
 
-lemma bcg_contrasim_contains_all_strat_consistent_atknodes:
+lemma cwg_contrasim_contains_all_strat_consistent_atknodes:
   assumes 
     \<open>contrasimulation R\<close>
     \<open>R p0 q0\<close>
@@ -106,24 +106,26 @@ next
     thus \<open>R p q\<close> using IH by simp
   next
     assume A: \<open>AttackerNode p q = (strategy_from_contrasim R (n0 # play))\<close>
-    have \<open>\<exists>A ppred. n0 = (DefenderNode A q ppred)\<close> using p0moved.hyps(3) 
-      strategy_from_contrasim.simps(1)[of \<open>R\<close>]
-      by (metis (no_types, lifting) A c_basic_game_node.inject(1) c_game_defender_node.elims(2))
-    then obtain A ppred where n0_def: \<open>n0 = (DefenderNode A q ppred)\<close> \<open>\<forall>a\<in>set A. a \<noteq> \<tau>\<close>
-      by (metis assms(3) c_basic_game.bcg_atknodes_precede_defnodes_in_plays
+    have \<open>\<exists>A ppred. n0 = (DefenderNode A q ppred)\<close> 
+      using p0moved.hyps(3) strategy_from_contrasim.simps(1)[of \<open>R\<close>]
+      by (metis (no_types, lifting) A c_word_game_node.inject(1) 
+          c_word_game_defender_node.elims(2))
+    then obtain A ppred where 
+      n0_def: \<open>n0 = (DefenderNode A q ppred)\<close> \<open>\<forall>a\<in>set A. a \<noteq> \<tau>\<close>
+      by (metis assms(3) c_word_game.cwg_atknodes_precede_defnodes_in_plays
           simulation_challenge p0moved.hyps(1, 3) strategy0_plays_subset)
     hence \<open>strategy_from_contrasim R (n0#play) =
         AttackerNode (SOME q1. R q1 q \<and> ppred \<Rightarrow>$ A  q1) q\<close> 
       using n0_def strategy_from_contrasim.simps(1)[of \<open>R\<close> \<open>A\<close> \<open>q\<close> \<open>ppred\<close> \<open>play\<close>] by auto
     hence p_def: \<open>p = (SOME p1. R p1 q \<and> ppred \<Rightarrow>$ A p1)\<close> using A by auto
-    have \<open>\<exists>qpred. hd play = (AttackerNode qpred ppred) \<and> c_game_moves (hd play) n0\<close> 
-      using bcg_atknodes_precede_defnodes_in_plays strategy0_plays_subset[OF p0moved.hyps(1)]
+    have \<open>\<exists>qpred. hd play = (AttackerNode qpred ppred) \<and> c_word_game_moves (hd play) n0\<close> 
+      using cwg_atknodes_precede_defnodes_in_plays strategy0_plays_subset[OF p0moved.hyps(1)]
       by (simp add: assms(3) n0_def  p0moved.hyps(3)) 
     then obtain qpred where qpred_def: \<open>hd play = (AttackerNode qpred ppred)\<close> 
-      and qpred_move: \<open>c_game_moves (hd play) n0\<close> by auto
+      and qpred_move: \<open>c_word_game_moves (hd play) n0\<close> by auto
     have qpred_q_move: \<open>qpred \<Rightarrow>$A q\<close> using qpred_def qpred_move n0_def by simp
     have \<open>hd play \<in> set (n0 # play)\<close> 
-      using bcg_second_play_elem_in_play_set strategy0_plays_subset[OF p0moved.hyps(1)] assms(3)
+      using cwg_second_play_elem_in_play_set strategy0_plays_subset[OF p0moved.hyps(1)] assms(3)
       by (auto simp add: n0_def)
     hence pred_R: \<open>R qpred ppred\<close> 
       by (simp add: qpred_def p0moved.hyps(1) p0moved.hyps(2))
@@ -144,14 +146,14 @@ next
   next
    assume A: \<open>AttackerNode p q = n1'\<close>
    from p1moved.hyps have \<open>player1_position n1\<close> by simp
-   hence \<open>c_game_defender_node n1'\<close>
-     by (metis c_game_defender_node.simps(2) c_game_moves.elims(2) p1moved.hyps(4))
+   hence \<open>c_word_game_defender_node n1'\<close>
+     by (metis c_word_game_defender_node.simps(2) c_word_game_moves.elims(2) p1moved.hyps(4))
    hence \<open>False\<close> using A by auto
    thus \<open>R p q\<close> ..
  qed
 qed
 
-lemma basic_contrasim_game_complete:
+lemma contrasim_word_game_complete:
   assumes 
     \<open>contrasimulation R\<close>
     \<open>R p q\<close> 
@@ -164,38 +166,39 @@ proof (safe)
   thus \<open>player1_wins_immediately play \<Longrightarrow> False\<close>
     unfolding player1_wins_immediately_def
   proof - 
-    assume A: \<open>c_game_defender_node (hd play) \<and> (\<nexists>p'. c_game_moves (hd play) p')\<close>
-    have player0_has_succ_node: \<open>c_game_defender_node (hd play) \<Longrightarrow>
-      \<exists>p'. c_game_moves (hd play) p'\<close>
+    assume A: \<open>c_word_game_defender_node (hd play) \<and> (\<nexists>p'. c_word_game_moves (hd play) p')\<close>
+    have player0_has_succ_node: \<open>c_word_game_defender_node (hd play) \<Longrightarrow>
+      \<exists>p'. c_word_game_moves (hd play) p'\<close>
     proof (induct rule: simple_game.plays_for_0strategy.induct[OF A1])
       case init: 1 
-      from assms(3) have \<open>\<not>c_game_defender_node (hd [initial])\<close> by simp
+      from assms(3) have \<open>\<not>c_word_game_defender_node (hd [initial])\<close> by simp
       hence \<open>False\<close> using init.prems by simp
       then show ?case ..
     next
       case p0moved: (2 n0 play)
-      from p0moved.hyps have \<open>c_game_defender_node n0\<close> by simp
+      from p0moved.hyps have \<open>c_word_game_defender_node n0\<close> by simp
       hence \<open>\<exists>A p1 q. n0 = (DefenderNode A p1 q)\<close>
-        by (meson c_game_defender_node.elims(2)) 
-      hence \<open>\<not>c_game_defender_node (strategy_from_contrasim R (n0#play))\<close>
-        using p0moved.hyps(4) c_game_moves.elims(2)[of \<open>n0\<close> \<open>strategy_from_contrasim R (n0#play)\<close>]
+        by (meson c_word_game_defender_node.elims(2)) 
+      hence \<open>\<not>c_word_game_defender_node (strategy_from_contrasim R (n0#play))\<close>
+        using p0moved.hyps(4) c_word_game_moves.elims(2)
+          [of \<open>n0\<close> \<open>strategy_from_contrasim R (n0#play)\<close>]
         by force 
       hence \<open>False\<close> using p0moved.prems by simp
       then show ?case ..
     next
       case p1moved: (3 n1 play n1')
-      hence \<open>\<not>c_game_defender_node n1\<close> using p1moved.hyps by simp
+      hence \<open>\<not>c_word_game_defender_node n1\<close> using p1moved.hyps by simp
       then obtain p q where n1_def: \<open>n1 = AttackerNode p q\<close>
-        using c_game_defender_node.elims(3) by auto
+        using c_word_game_defender_node.elims(3) by auto
       hence pq_in_R: \<open>R p q\<close> 
-        using bcg_contrasim_contains_all_strat_consistent_atknodes[OF assms,
+        using cwg_contrasim_contains_all_strat_consistent_atknodes[OF assms,
                 of \<open>n1#play\<close>, OF p1moved.hyps(1)] 
         by auto
-      have is_def: \<open>c_game_defender_node n1'\<close> using p1moved.prems by auto
+      have is_def: \<open>c_word_game_defender_node n1'\<close> using p1moved.prems by auto
       then obtain A p1 q0 where n1'_def: \<open>n1' = DefenderNode A p1 q0\<close>
-        using c_game_defender_node.elims(2)[OF is_def] by auto
+        using c_word_game_defender_node.elims(2)[OF is_def] by auto
       hence \<open>\<forall>a\<in>set A. a \<noteq> \<tau>\<close> using p1moved.hyps(4) n1_def by simp
-      have Move_n1_n1': \<open>c_game_moves (AttackerNode p q) (DefenderNode A p1 q0)\<close> 
+      have Move_n1_n1': \<open>c_word_game_moves (AttackerNode p q) (DefenderNode A p1 q0)\<close> 
         using p1moved.hyps n1_def n1'_def by auto
       hence same_q: \<open>q0 = q\<close> by auto
       from Move_n1_n1' have p_succ: \<open>p \<Rightarrow>$A p1\<close> by auto
@@ -205,7 +208,7 @@ proof (safe)
         unfolding contrasimulation_def by auto
       hence \<open>\<exists> q'. (q \<Rightarrow>$ A q')\<and> R q' p1\<close>
         using Contra[OF \<open>\<forall>a\<in>set A. a \<noteq> \<tau>\<close> pq_in_R p_succ] by auto
-      hence \<open>\<exists> p1 q1. c_game_moves n1' (AttackerNode p1 q1)\<close>
+      hence \<open>\<exists> p1 q1. c_word_game_moves n1' (AttackerNode p1 q1)\<close>
         using same_q n1'_def by auto
       then show ?case by auto
     qed
@@ -213,9 +216,9 @@ proof (safe)
   qed
 qed
 
-subsection \<open>Winning Strategy Implies Contrasimulation (Soundness)\<close>
+subsection \<open>Winning Strategy Implies Contrasimulation in Word Game (Soundness)\<close>
 
-lemma bcg_strategy_from_contrasim_sound: 
+lemma cwg_strategy_from_contrasim_sound: 
   assumes
     \<open>R p0 q0\<close>
     \<open>contrasimulation R\<close>
@@ -227,17 +230,19 @@ proof (safe)
   fix n0 play
   assume A:
     \<open>n0 # play \<in> plays_for_0strategy (strategy_from_contrasim R) initial\<close>
-    \<open>c_game_defender_node n0\<close>
+    \<open>c_word_game_defender_node n0\<close>
   then obtain A p1 q where n0_def: \<open>n0 = DefenderNode A p1 q\<close>
-    using c_game_defender_node.elims(2) by blast 
+    using c_word_game_defender_node.elims(2) by blast 
   then obtain p where p_def: \<open>hd play = AttackerNode p q\<close>
-    using n0_def A bcg_atknodes_precede_defnodes_in_plays assms(3) strategy0_plays_subset by blast
-  hence \<open>c_game_moves (AttackerNode p q) (DefenderNode A p1 q)\<close> 
-    using A n0_def by (metis assms(3) bcg_atknodes_precede_defnodes_in_plays strategy0_plays_subset)
+    using n0_def A cwg_atknodes_precede_defnodes_in_plays assms(3) strategy0_plays_subset 
+    by blast
+  hence \<open>c_word_game_moves (AttackerNode p q) (DefenderNode A p1 q)\<close> 
+    using A n0_def 
+    by (metis assms(3) cwg_atknodes_precede_defnodes_in_plays strategy0_plays_subset)
   hence mov_p_p1: \<open>p \<Rightarrow>$A p1\<close> \<open>\<forall>a\<in>set A. a \<noteq> \<tau>\<close> by auto  
   from p_def have \<open>R p q\<close> 
-    using bcg_contrasim_contains_all_strat_consistent_atknodes A assms
-      bcg_second_play_elem_in_play_set n0_def strategy0_plays_subset
+    using cwg_contrasim_contains_all_strat_consistent_atknodes A assms
+      cwg_second_play_elem_in_play_set n0_def strategy0_plays_subset
     by fastforce
   with mov_p_p1 have q1_def: \<open>\<exists>q1. R q1 p1 \<and> q \<Rightarrow>$A q1\<close> 
     using assms(2) unfolding contrasimulation_def by blast
@@ -249,11 +254,11 @@ proof (safe)
     \<open>AttackerNode (SOME q1 . R q1 p1 \<and> q \<Rightarrow>$A q1) p1 = AttackerNode q' p1\<close> by blast
   hence q'_def: \<open>q' = (SOME q1 . R q1 p1 \<and> q \<Rightarrow>$A q1)\<close> by auto
   with someI_ex[OF q1_def] have \<open>R q' p1 \<and> q \<Rightarrow>$A q'\<close> by blast
-  thus \<open>c_game_moves n0 (strategy_from_contrasim R (n0 # play))\<close>
+  thus \<open>c_word_game_moves n0 (strategy_from_contrasim R (n0 # play))\<close>
     using q'_def by (simp add: n0_def) 
 qed
 
-lemma basic_contrasim_game_sound: 
+lemma contrasim_word_game_sound: 
   assumes
     \<open>player0_winning_strategy f initial\<close>
     \<open>sound_0strategy f initial\<close>
@@ -271,9 +276,11 @@ proof (safe)
     \<open>play \<in> plays_for_0strategy f initial \<and> hd play = AttackerNode p q\<close> ..
   from assms(1) have \<open>\<not>player1_wins_immediately play\<close>
     using player0_winning_strategy_def play_def by auto
-  hence \<open>(c_game_defender_node (hd play) \<and> (\<nexists>p'. c_game_moves (hd play) p')) \<Longrightarrow> False\<close> 
+  hence \<open>(c_word_game_defender_node (hd play) \<and> (\<nexists>p'. c_word_game_moves (hd play) p')) 
+    \<Longrightarrow> False\<close> 
     using player1_wins_immediately_def by auto
-  hence Def_not_stuck: \<open>c_game_defender_node (hd play) \<Longrightarrow> (\<nexists>p'. c_game_moves (hd play) p')
+  hence Def_not_stuck: 
+    \<open>c_word_game_defender_node (hd play) \<Longrightarrow> (\<nexists>p'. c_word_game_moves (hd play) p')
     \<Longrightarrow> False\<close> 
     by auto
   have \<open>(p \<Rightarrow>$A p1) \<Longrightarrow> (((DefenderNode A p1 q)#play) \<in> plays_for_0strategy f initial)\<close>
@@ -284,7 +291,7 @@ proof (safe)
       by (metis hd_Cons_tl play_def strategy0_plays_subset no_empty_plays) 
     hence inF:\<open>(hd play)#(tl play) \<in> plays_for_0strategy f initial\<close> by (simp add: play_def)
     have pl1: \<open>player1_position (hd play)\<close> by (simp add: play_def)
-    have mov0:\<open>c_game_moves (hd play) (DefenderNode A p1 q)\<close> 
+    have mov0:\<open>c_word_game_moves (hd play) (DefenderNode A p1 q)\<close> 
       using  \<open>\<forall>a\<in>set A. a \<noteq> \<tau>\<close> by (auto simp add: play_def A1)
     have \<open>(DefenderNode A p1 q)#(hd play)#(tl play) \<in> plays_for_0strategy f initial\<close> 
       using plays_for_0strategy.p1move[OF inF pl1 mov0] .
@@ -295,25 +302,25 @@ proof (safe)
     by (simp add: A1)
   hence \<open>\<not>(player1_wins_immediately (DefenderNode A p1 q#play))\<close> 
     using assms(1) player0_winning_strategy_def by auto
-  hence \<open>\<exists>n1. c_game_moves (DefenderNode A p1 q) n1\<close>
+  hence \<open>\<exists>n1. c_word_game_moves (DefenderNode A p1 q) n1\<close>
     using player1_wins_immediately_def by auto
-  have move_ex: \<open>c_game_moves (DefenderNode A p1 q) (f (DefenderNode A p1 q # play))\<close>
+  have move_ex: \<open>c_word_game_moves (DefenderNode A p1 q) (f (DefenderNode A p1 q # play))\<close>
     using assms(2) def_in_f sound_0strategy_def by auto
   hence in_f: \<open>f ((DefenderNode A p1 q) # play) # (DefenderNode A p1 q) # play
       \<in> plays_for_0strategy f initial\<close> 
     using plays_for_0strategy.p0move[OF def_in_f] by auto
   obtain n1 where
     n1_def: \<open>n1 = f (DefenderNode A p1 q # play)\<close> and
-    n1_move: \<open>c_game_moves (DefenderNode A p1 q) n1\<close>
+    n1_move: \<open>c_word_game_moves (DefenderNode A p1 q) n1\<close>
     using move_ex by auto
   hence \<open>\<exists>q1. n1 = (AttackerNode q1 p1)\<close>
-    using c_game_moves.elims(2)[of \<open>DefenderNode A p1 q\<close> n1] by auto
+    using c_word_game_moves.elims(2)[of \<open>DefenderNode A p1 q\<close> n1] by auto
   from this obtain q1 where
     q1_def: \<open>n1 = (AttackerNode q1 p1)\<close> ..
-  have \<open>c_game_moves (DefenderNode A p1 q) (AttackerNode q1 p1)\<close>
+  have \<open>c_word_game_moves (DefenderNode A p1 q) (AttackerNode q1 p1)\<close>
     using q1_def move_ex n1_def by auto
-  hence q1_succ: \<open>q \<Rightarrow>$A q1\<close> using c_game_moves.simps(2) by auto
-  have def: \<open>c_game_defender_node (DefenderNode A p1 q)\<close> by simp
+  hence q1_succ: \<open>q \<Rightarrow>$A q1\<close> using c_word_game_moves.simps(2) by auto
+  have def: \<open>c_word_game_defender_node (DefenderNode A p1 q)\<close> by simp
   hence \<open>(AttackerNode q1 p1)#(DefenderNode A p1 q)#play \<in> plays_for_0strategy f initial\<close>
     using q1_def n1_def in_f by auto
   then obtain R_play where
@@ -324,7 +331,7 @@ proof (safe)
   thus \<open>R p q \<Longrightarrow> p \<Rightarrow>$ A  p1 \<Longrightarrow> \<exists>q1. q \<Rightarrow>$ A  q1 \<and> R q1 p1\<close> using q1_succ by auto
 qed
 
-theorem winning_strategy_in_basic_game_iff_contrasim:
+theorem winning_strategy_in_c_word_game_iff_contrasim:
   assumes
     \<open>initial = AttackerNode p q\<close>
   shows 
@@ -336,7 +343,7 @@ proof
   then obtain f where
     \<open>contrasimulation (\<lambda>p q.
       \<exists>play\<in>plays_for_0strategy f initial. hd play = AttackerNode p q)\<close>
-    using basic_contrasim_game_sound by blast
+    using contrasim_word_game_sound by blast
   moreover have
     \<open>(\<lambda>p q. \<exists>play\<in>plays_for_0strategy f initial. hd play = AttackerNode p q) p q\<close>
     using assms plays_for_0strategy.init[of _ f] by (meson list.sel(1))
@@ -345,8 +352,8 @@ next
   assume
     \<open>\<exists> C. contrasimulation C \<and> C p q\<close>
   thus \<open>(\<exists>f. player0_winning_strategy f initial \<and> sound_0strategy f initial)\<close>
-    using basic_contrasim_game_complete[OF _ _ assms]
-         bcg_strategy_from_contrasim_sound[OF _ _ assms] by blast
+    using contrasim_word_game_complete[OF _ _ assms]
+         cwg_strategy_from_contrasim_sound[OF _ _ assms] by blast
 qed
 
 end                         
